Change postcondition definitions to accept functions with return values

src/Lib/Notations.v
@@ -43,23 +43,35 @@ Infix "~>" := scalar (at level 40, only parsing).
 
 Notation "[[ locals ]]" := ({| value := locals; _value_ok := _ |}) (only printing).
 
-(* TODO: rets are not always nil!! *)
 Definition postcondition_for
-           {semantics : Semantics.parameters} spec R tr :=
+           {semantics : Semantics.parameters} spec R tr rets_ok :=
   (fun (tr' : Semantics.trace) (mem' : Semantics.mem) (rets : list address) =>
-     tr = tr' /\ rets = nil
+     tr = tr' /\ rets_ok rets
      /\ sep spec R mem').
 
 Definition postcondition_norets
            {semantics : Semantics.parameters} locals_post spec R tr :=
   (fun (tr' : Semantics.trace) (mem' : Semantics.mem) (locals : Semantics.locals) =>
-     locals_post locals /\ postcondition_for spec R tr tr' mem' []).
+     locals_post locals
+     /\ postcondition_for spec R tr (fun r => r = nil) tr' mem' []).
+
+Definition postcondition_withrets
+           {semantics : Semantics.parameters} locals_post spec R tr rets :=
+  (fun (tr' : Semantics.trace) (mem' : Semantics.mem) (locals : Semantics.locals) =>
+     locals_post locals
+     /\ postcondition_for spec R tr (fun r => r = rets) tr' mem' rets).
 
 Notation "'find' body 'implementing' spec 'and-locals-post' locals_post 'with-locals' locals 'and-memory' mem 'and-trace' tr 'and-rest' R 'and-functions' fns" :=
   (WeakestPrecondition.cmd
      (WeakestPrecondition.call fns)
      body tr mem locals
      (postcondition_norets locals_post spec R tr)) (at level 0).
+
+Notation "'find' body 'implementing' spec 'and-returning' rets 'and-locals-post' locals_post 'with-locals' locals 'and-memory' mem 'and-trace' tr 'and-rest' R 'and-functions' fns" :=
+  (WeakestPrecondition.cmd
+     (WeakestPrecondition.call fns)
+     body tr mem locals
+     (postcondition_withrets locals_post spec R tr rets)) (at level 0).
 
 Notation "'liftexists' x .. y ',' P" :=
   (Lift1Prop.ex1
@@ -71,6 +83,18 @@ Notation "'liftexists' x .. y ',' P" :=
 
 (* precondition is more permissively handled than postcondition in order to
    non-separation-logic (or multiple separation-logic) preconditions *)
+Notation "'forall!' x .. y ',' pre '===>' fname '@' args 'returns' rets '===>' post" :=
+(fun functions =>
+   (forall x,
+       .. (forall y,
+              forall R tr mem,
+                pre R mem ->
+                WeakestPrecondition.call
+                  functions fname tr mem args
+                  (postcondition_for post R tr (fun r => r = rets))) ..))
+     (x binder, y binder, only parsing, at level 199).
+
+(* shorthand for no return values *)
 Notation "'forall!' x .. y ',' pre '===>' fname '@' args '===>' post" :=
 (fun functions =>
    (forall x,
@@ -79,5 +103,6 @@ Notation "'forall!' x .. y ',' pre '===>' fname '@' args '===>' post" :=
                 pre R mem ->
                 WeakestPrecondition.call
                   functions fname tr mem args
-                  (postcondition_for post R tr)) ..))
+                  (postcondition_for post R tr (fun r => r = nil))) ..))
      (x binder, y binder, only parsing, at level 199).
+
