src/Examples/Cells/Swap.v
@@ -22,7 +22,7 @@ Derive swap_body SuchThat
              (swap :: functions)
              "swap"
              tr mem [a_ptr;b_ptr]
-             (postcondition_for (TwoCells a_ptr b_ptr (swap_gallina_spec a b)) R tr)))
+             (postcondition_for (TwoCells a_ptr b_ptr (swap_gallina_spec a b)) R tr (fun r => r = nil))))
   As swap_body_correct.
 Proof.
   compile.
